common/words2.ml
@@ -98,6 +98,85 @@ let numbit = new_definition `numbit i n = ODD(n DIV (2 EXP i))`;;
 let NUMBIT_VAL = prove (`numbit i (val (e:N word)) = bit i e`,
   REWRITE_TAC [numbit; BIT_VAL]);;
 
+let NUMBIT_BINARY_DIGITSUM = prove
+ (`!s b k.
+      FINITE s
+      ==> (numbit k (nsum s (\i. 2 EXP i * bitval (b i))) <=> k IN s /\ b k)`,
+  SIMP_TAC[numbit; ODD_MOD; DIGITSUM_DIV_MOD; BITVAL_BOUND_ALT] THEN
+  REPEAT GEN_TAC THEN COND_CASES_TAC THEN ASM_REWRITE_TAC[bitval] THEN
+  ARITH_TAC);;
+
+let NUMBIT_ADD_SHIFT = prove
+ (`!a b i e. a < 2 EXP e
+             ==> numbit i (a + 2 EXP e * b) =
+                 (if i < e then numbit i a else numbit (i - e) b)`,
+  REPEAT STRIP_TAC THEN REWRITE_TAC[numbit] THEN COND_CASES_TAC THENL
+   [SUBGOAL_THEN `e = i + SUC(e - i - 1)` SUBST1_TAC THENL
+     [ASM_ARITH_TAC; REWRITE_TAC[EXP_ADD; GSYM MULT_ASSOC]] THEN
+    SIMP_TAC[DIV_MULT_ADD; EXP_EQ_0; ARITH_EQ] THEN
+    REWRITE_TAC[ODD_ADD; ODD_MULT; ODD_EXP; ARITH_ODD; ARITH_EVEN; NOT_SUC];
+    SUBGOAL_THEN `i:num = e + (i - e)` SUBST1_TAC THENL
+     [ASM_ARITH_TAC; REWRITE_TAC[EXP_ADD; GSYM DIV_DIV]] THEN
+    SIMP_TAC[DIV_MULT_ADD; EXP_EQ_0; ARITH_EQ] THEN
+    ASM_SIMP_TAC[DIV_LT; ADD_CLAUSES; ONCE_REWRITE_RULE[ADD_SYM] ADD_SUB]]);;
+
+let NUMBIT_0 = prove
+ (`!i. ~(numbit i 0)`,
+  REWRITE_TAC[numbit; DIV_0; ODD]);;
+
+let NUMBIT_SHIFT = prove
+ (`!b i e. numbit i (2 EXP e * b) <=> e <= i /\ numbit (i - e) b`,
+  MP_TAC(SPEC `0` NUMBIT_ADD_SHIFT) THEN
+  REWRITE_TAC[EXP_LT_0; ARITH_EQ; ADD_CLAUSES; NUMBIT_0] THEN
+  MESON_TAC[NOT_LT]);;
+
+let NUMBIT_DIV_EXP = prove
+ (`!j k p. numbit j (k DIV 2 EXP p) <=> numbit (j + p) k`,
+  REWRITE_TAC[numbit; DIV_DIV; GSYM EXP_ADD] THEN REWRITE_TAC[ADD_SYM]);;
+
+let NUMBIT_MOD_EXP = prove
+ (`!j k p. numbit j (k MOD 2 EXP p) <=> j < p /\ numbit j k`,
+  REPEAT STRIP_TAC THEN ASM_CASES_TAC `j:num < p` THEN
+  ASM_REWRITE_TAC[numbit] THENL
+   [REWRITE_TAC[DIV_MOD; ONCE_REWRITE_RULE[MULT_SYM] (GSYM(CONJUNCT2 EXP));
+                ODD_MOD; MOD_MOD_EXP_MIN] THEN
+    ASM_SIMP_TAC[ARITH_RULE `i < n ==> MIN n (SUC i) = SUC i`];
+    MATCH_MP_TAC(MESON[ODD] `n = 0 ==> ~ODD n`) THEN
+    MATCH_MP_TAC DIV_LT THEN TRANS_TAC LTE_TRANS `2 EXP p` THEN
+    ASM_SIMP_TAC[DIVISION; LE_EXP; EXP_EQ_0; ARITH_EQ] THEN
+    ASM_REWRITE_TAC[GSYM NOT_LT]]);;
+
+let NUMBIT_MUL2 = prove
+ (`!j k. numbit j (2 * k) <=> 1 <= j /\ numbit (j - 1) k`,
+  REWRITE_TAC[GSYM NUMBIT_SHIFT; EXP_1]);;
+
+let NUMBIT_DIV2 = prove
+ (`!j k. numbit j (k DIV 2) <=> numbit (j + 1) k`,
+  REWRITE_TAC[GSYM NUMBIT_DIV_EXP; EXP_1]);;
+
+let NUMBIT_MOD2 = prove
+ (`!j k. numbit j (k MOD 2) <=> j = 0 /\ numbit j k`,
+  REWRITE_TAC[ARITH_RULE `j = 0 <=> j < 1`; GSYM NUMBIT_MOD_EXP; EXP_1]);;
+
+let BINARY_DIGITSUM_NUMBITS = prove
+ (`!n k. nsum {i | i < k} (\i. 2 EXP i * bitval(numbit i n)) =
+         n MOD (2 EXP k)`,
+  REWRITE_TAC[numbit; BITVAL_ODD; DIGITSUM_WORKS_GEN]);;
+
+let NUMBITS_EQ = prove
+ (`!m n. (!i. numbit i m = numbit i n) <=> m = n`,
+  MATCH_MP_TAC WLOG_LT THEN REWRITE_TAC[] THEN
+  CONJ_TAC THENL [REWRITE_TAC[EQ_SYM_EQ]; SIMP_TAC[LT_IMP_NE]] THEN
+  MAP_EVERY X_GEN_TAC [`m:num`; `n:num`] THEN REPEAT STRIP_TAC THEN
+  MP_TAC(ISPECL [`m:num`; `n:num`] BINARY_DIGITSUM_NUMBITS) THEN
+  MP_TAC(ISPECL [`n:num`; `n:num`] BINARY_DIGITSUM_NUMBITS) THEN
+  ASM_REWRITE_TAC[] THEN DISCH_THEN SUBST1_TAC THEN
+  MATCH_MP_TAC(ARITH_RULE
+   `n MOD 2 EXP n = n /\ m MOD 2 EXP n = m /\ m < n
+    ==> ~(n MOD 2 EXP n = m MOD 2 EXP n)`) THEN
+  ASM_REWRITE_TAC[] THEN CONJ_TAC THEN MATCH_MP_TAC MOD_LT THEN
+  ASM_MESON_TAC[LT_POW2_REFL; LT_TRANS]);;
+
 (* * BIT_PRED `i` returns (None, `|- i = _0`) or (Some(`j`), `|- i = SUC j`)
      if `i` is a raw numeral (a numeral without the initial `NUMERAL`).
    * NUMBIT_CONV `numbit n i` proves `numbit n i = T` or `numbit n i = F` if
